examples/safeRemotePurchase/PurchaseLiquid.v
@@ -1,0 +1,17 @@
+Require Import Purchase.
+Require Import BuildUtils.
+Require Import Automation.
+From Coq Require Import ZArith.
+Require Import Serializable.
+Require Import Blockchain.
+Require Import Containers.
+Require Import Extras.
+Require Import RecordUpdate.
+From Coq Require Import Bool.
+From Coq Require Import Lia.
+From Coq Require Import List.
+Import ListNotations.
+From Coq Require Import Permutation.
+Require Import ChainedList.
+Require Import Strat.
+Require Import FMapList.
