README.md
@@ -1,3 +1,5 @@
 # coq_liquidity
 
 My postgraduate research project Coq verification code
+
+Require : Windows 11 Coq 8.16.1
